---
title: "Answer"
---

Given
\begin{align}
    f(t) &= e^{t}\roundbr{u(t) - u(t - \pi/2)}\newline
    L(f) &= L\roundbr{e^{t - 0}u^{t - 0}} - L\roundbr{e^{t}u\roundbr{t - \frac{\pi}{2}}}\newline
    &= e^{0s}\frac{1}{s-1} - e^{-\frac{\pi}{2}s}L\roundbr{e^{t + \pi/2}}\newline
    &= \frac{1}{s-1} - e^{-\frac{\pi}{2}s}e^{\pi/2}L\roundbr{e^{t}}\newline
    &= \frac{1}{s-1} - e^{-\frac{\pi}{2}s}e^{\pi/2}\frac{1}{s-1}\newline
    &= \frac{1 - e^{-\frac{\pi}{2} (s-1)}}{s-1}
\end{align}

using two different versions of the second shift theorem.
