---
title: "Answer"
---

Taking the reciprocal on both sides,
\begin{align}
    \frac{dx}{dy} &= 6e^{y} - 2x\newline
    \implies \diffone{x} + 2x &= 6e^{y}\newline
\end{align}
which is a linear differential equation. Considering the integrating factor as $exp \roundbr{\int 2dy} = exp \roundbr{2y}$,
\begin{align}
    \implies \diffone{x}e^{2y} + 2xe^{2y} &= 6e^{3y}\newline
    \frac{d}{dy} \roundbr{xe^{2y}} &= 6e^{3y}\newline
    xe^{2y} &= \int 6e^{3y}dy + c = 2e^{3y} + c
\end{align}

Another problem leveraging is the same transformation is
\begin{align}
    \roundbr{y^{2} + 2x}\frac{dy}{dx} = y
\end{align}
