---
title: "Answer"
---

Rearranging the equation, we have
\begin{align}
    \frac{dy}{dx} &= \frac{1 + y^{2}}{\tan^{-1} y - x}
\end{align}

This equation is not readily solvable. However, we can instead try to get $x$ a function of $y$ by inverting the above equation
\begin{align}
    \frac{dx}{dy} &= \frac{\tan^{-1} y - x}{1 + y^{2}}\newline
    &= \frac{\tan^{-1} y}{1 + y^{2}} - \frac{1}{1 + y^{2}}x\newline
    \implies \frac{dx}{dy} + \frac{1}{1 + y^{2}}x &= \frac{\tan^{-1} y}{1 + y^{2}}
\end{align}

Which is a linear equation. The integrating factor is
\begin{align}
    IF &= e^{\int \frac{1}{1 + y^{2}}dy} = e^{\tan^{-1} y}\newline
    \implies e^{\tan^{-1} y}\frac{dx}{dy} + \frac{e^{\tan^{-1} y}}{1 + y^{2}}x &= \frac{e^{\tan^{-1} y}\tan^{-1} y}{1 + y^{2}}\newline
    xe^{\tan^{-1} y} &= \int \frac{e^{\tan^{-1} y}\tan^{-1} y}{1 + y^{2}} dy\newline
\end{align}

Substituiting $\tan^{-1} y = v$
\begin{align}
    \frac{1}{1 + y^{2}}dy &= dv\newline
    \implies \int \frac{e^{\tan^{-1} y}\tan^{-1} y}{1 + y^{2}} &= \int te^{t}dt\newline
    &= te^{t} - e^{t} + c\newline
    &= e^{\tan^{-1} y}\tan^{-1} y - e^{\tan^{-1} y} + c
\end{align}

Thus,
\begin{align}
    xe^{\tan^{-1} y} &= e^{\tan^{-1} y}\tan^{-1} y - e^{\tan^{-1} y} + c\newline
    \implies x &= \tan^{-1} y - 1 + ce^{-\tan^{-1} y}
\end{align}
