---
title: "Answer"
---

We first solve the homogenous equation by substituiting $x^{m}$ as the solution (this is an Euler-Cauchy equation)
\begin{align}
    x^{3}\diffthree{y} - 3x^{2}\difftwo{y} + 6x\diffone{y} - 6y &= 0\newline
    x^{3}m(m-1)(m-2)x^{m-3} - 3x^{2}m(m-1)x^{m-2} + 6xmx^{m-1} - 6x^{m} &= 0\newline
    \implies m(m-1)(m-2) -3m(m-1) + 6m - 6 &= 0\newline
    m^{3} - 6m^{2} + 11m - 6 &= 0\newline
    m &= 1, 2, 3
\end{align}
Root 1 is easily identifiable by inspection. Remaining roots can be obtained by factorization. Hence, $y_{h}$ is
\begin{align}
    y_{h} &= c_{1}x + c_{2}x^{2} + c_{3}x^{3}
\end{align}
with $x$, $x^{2}$ and $x^{3}$ as the bases. Since $r(x)$ is not a standard function (for method of undetermined coefficients), we will try to use variation of parameters to solve for $y_{p}$
\begin{align}
    W &= \detm{\begin{matrix}
        x &x^{2} &x^{3}\newline
        1 &2x &3x^{2}\newline
        0 &2 &6x
    \end{matrix}} = 2x^{3}
\end{align}
Hence, all $W_{i}$ are
\begin{align}
    W_{1} &= \detm{\begin{matrix}
        0 &x^{2} &x^{3}\newline
        0 &2x &3x^{2}\newline
        1 &2 &6x
    \end{matrix}} = x^{4}\newline
    W_{2} &= \detm{\begin{matrix}
        x &0 &x^{3}\newline
        1 &0 &3x^{2}\newline
        0 &1 &6x
    \end{matrix}} = -2x^{3}\newline
    W_{3} &= \detm{\begin{matrix}
        x &x^{2} &0\newline
        1 &2x &0\newline
        0 &2 &1
    \end{matrix}} = x^{2}
\end{align}
Now, to apply the method of undetermined, we also convert our equation to the standard form
\begin{align}
    \diffthree{y} - \frac{3}{x}\difftwo{y} + \frac{6}{x^{2}}\diffone{y} - \frac{6}{x^{3}}y = x\ln x
\end{align}
\begin{align}
    y_{p}(x) &= \sum_{k=1}^{n}y_{k}(x)\int \frac{W_{k}(x)}{W(x)}r(x)dx\newline
    &= x\int\frac{x^{4}}{2x^{3}}x\ln x dx + x^{2}\int\frac{-2x^{3}}{2x^{3}}x\ln x dx + x^{3}\int\frac{x^{2}}{2x^{3}}x\ln x dx\newline
    &= \frac{x}{2}\roundbr{\frac{x^{3}}{3}\ln x - \frac{x^{3}}{9}} - x^{2}\roundbr{\frac{x^{2}}{2}\ln x - \frac{x^{2}}{4}} + \frac{x^{3}}{2}\roundbr{x\ln x - x}\newline
    &= \frac{x^{4}}{6}\ln x - \frac{11}{36}x^{4}
\end{align}
Thus, the general solution is
\begin{align}
    y = c_{1}x + c_{2}x^{2} + c_{3}x^{3} + \frac{x^{4}}{6}\roundbr{\ln x - \frac{11}{6}}
\end{align}
