\documentclass[../../probability-notes.tex]{subfiles}
\begin{document}
    We first begin by calculating the posterior of $\theta$ given observations
    \begin{align*}
        f(\theta|X_{1}, X_{2}, \ldots, X_{n}) &= \frac{f(X_{1}, X_{2}, \ldots, X_{n}|\theta)p(\theta)}{\int f(X_{1}, X_{2}, \ldots, X_{n}|\theta)p(\theta) d\theta}\\
        f(X_{1}, X_{2}, \ldots, X_{n}|\theta) &= \frac{1}{\sqrt{2 \pi \sigma_{0}^{2}}} exp(-\frac{\sum_{i=1}^{n} (X_{i} - \theta)^{2}}{2\sigma_{0}^{2}})\\
        p(\theta) &= \frac{1}{\sqrt{2 \pi \sigma^{2}}} exp(-\frac{(\theta - \mu)^{2}}{2\sigma^{2}})\\
        f(X_{1}, X_{2}, \ldots, X_{n}|\theta)p(\theta) &= \frac{1}{2 \pi \sigma_{0} \sigma} exp(-\frac{\sum_{i=1}^{n} (X_{i} - \theta)^{2}}{2\sigma_{0}^{2}} -\frac{(\theta - \mu)^{2}}{2\sigma^{2}})\\
        \frac{\sum_{i=1}^{n} (X_{i} - \theta)^{2}}{2\sigma_{0}^{2}} +\frac{(\theta - \mu)^{2}}{2\sigma^{2}} &= \frac{\theta^{2}(\sigma_{0}^{2} + n\sigma^{2}) - 2\theta(\sigma_{0}^{2} \mu + \sigma^{2} \sum_{i=1}^{n} X_{i}) + (\sigma_{0}^{2} \mu^{2} + \sigma^{2} \sum_{i=1}^{n}X_{i}^{2})}{2\sigma_{0}^{2}\sigma^{2}}\\
        &= \frac{\big(\theta - \frac{\sigma_{0}^{2} \mu + \sigma^{2}\sum_{i=1}^{n} X_{i}}{\sigma_{0}^{2} + n\sigma^{2}}\big)^{2} + \big(\frac{\sigma_{0}^{2} \mu^{2} + \sigma^{2} \sum_{i=1}^{n}X_{i}^{2}}{\sigma_{0}^{2} + n\sigma^{2}} - \big(\frac{\sigma_{0}^{2} \mu + \sigma^{2}\sum_{i=1}^{n} X_{i}}{\sigma_{0}^{2} + n\sigma^{2}}\big)^{2}\big)}{(2\sigma_{0}^{2} \sigma^{2})/(\sigma_{0}^{2} + n\sigma^{2})}\\
        f(X_{1}, X_{2}, \ldots, X_{n}|\theta)p(\theta) &= \bigg(\frac{1}{2\sigma_{0}\sigma}exp\bigg(\frac{\big(\frac{\sigma_{0}^{2} \mu^{2} + \sigma^{2} \sum_{i=1}^{n}X_{i}^{2}}{\sigma_{0}^{2} + n\sigma^{2}} - \big(\frac{\sigma_{0}^{2} \mu + \sigma^{2}\sum_{i=1}^{n} X_{i}}{\sigma_{0}^{2} + n\sigma^{2}}\big)^{2}\big)}{2\sigma_{0}^{2} \sigma^{2})/(\sigma_{0}^{2} + n\sigma^{2})}\bigg)\times\\
        &\bigg(\frac{1}{\sqrt{2\pi(2\sigma_{0}^{2} \sigma^{2})/(\sigma_{0}^{2} + n\sigma^{2})}}exp\bigg(-\frac{\big(\theta - \frac{\sigma_{0}^{2} \mu + \sigma^{2}\sum_{i=1}^{n} X_{i}}{\sigma_{0}^{2} + n\sigma^{2}}\big)^{2}}{2\sigma_{0}^{2} \sigma^{2}/(\sigma_{0}^{2} + n\sigma^{2})}\bigg)\bigg)\\
        &= C \times \mathcal{N}\bigg(\frac{\sigma_{0}^{2} \mu + \sigma^{2}\sum_{i=1}^{n} X_{i}}{\sigma_{0}^{2} + n\sigma^{2}}, \frac{2\sigma_{0}^{2} \sigma^{2}}{\sigma_{0}^{2} + n\sigma^{2}}\bigg)\\
        f(\theta|X_{1}, X_{2}, \ldots, X_{n}) &= \frac{C \times \mathcal{N}\bigg(\frac{\sigma_{0}^{2} \mu + \sigma^{2}\sum_{i=1}^{n} X_{i}}{\sigma_{0}^{2} + n\sigma^{2}}, \frac{2\sigma_{0}^{2} \sigma^{2}}{\sigma_{0}^{2} + n\sigma^{2}}\bigg)}{C \times \int_{-\inf}^{\inf} \mathcal{N}\bigg(\frac{\sigma_{0}^{2} \mu + \sigma^{2}\sum_{i=1}^{n} X_{i}}{\sigma_{0}^{2} + n\sigma^{2}}, \frac{2\sigma_{0}^{2} \sigma^{2}}{\sigma_{0}^{2} + n\sigma^{2}}\bigg) d\theta}\\
        &= \mathcal{N}\bigg(\frac{\sigma_{0}^{2} \mu + \sigma^{2}\sum_{i=1}^{n} X_{i}}{\sigma_{0}^{2} + n\sigma^{2}}, \frac{2\sigma_{0}^{2} \sigma^{2}}{\sigma_{0}^{2} + n\sigma^{2}}\bigg)\\
        &= \mathcal{N}\bigg(\frac{\sigma_{0}^{2} \mu + n\sigma^{2}\overline{X}}{\sigma_{0}^{2} + n\sigma^{2}}, \frac{2\sigma_{0}^{2} \sigma^{2}}{\sigma_{0}^{2} + n\sigma^{2}}\bigg)
    \end{align*}
    or, the new estimate of the mean is the weighted sum of the prior mean and the estimated mean from the observations, with the weights being proportional to the inverse of the standard deviations. The new standard deviation is also the geometric mean of the original standard deviations.
\end{document}