\documentclass[../../probability-notes.tex]{subfiles}
\begin{document}
        This quantity can be calculated using the law of total expectation
        \begin{align*}
            E[X] = E[X|A_{1}]P(A_{1}) + E[X|A_{2}]P(A_{2}) + \cdots + E[X|A_{n}]P(A_{n}) \tag*{where $A_{i}$ are disjoint}
        \end{align*}
        Let $H_{1}$ denote heads at first toss, $H_{2}$ denote heads at the second toss, $T_{1}$ denote tails at first toss and $T_{2}$ denote tails at the second toss. Then,
        \begin{align*}
            E[X] &= E[X|H_{1}]P(H_{1}) + E[X|T_{1}]P(T_{1})\\
            E[X|H_{1}] &= E[X|H_{1}H_{2}]P(H_{2}|H_{1}) + E[X|H_{1}T_{2}]P(T_{2}|H_{1})\\
                    &= 2p + (1 + E[X|T_{1}])(1-p)\\
            E[X|T_{1}] &= E[X|T_{1}T_{2}]P(T_{2}|T_{1}) + E[X|T_{1}H_{2}]P(H_{2}|T_{1})\\
                    &= 2(1-p) + (1 + E[X|H_{1}])p\\
        \end{align*}
        $E[X|H_{1}T_{2}] = 1 + E[X|T_{1}]$ because the tails after the first heads implies the first heads is now irrelevant and we have wasted one toss on the heads. The remaining process is same as starting from the first coin toss as tails. \newline
        Solving for the conditional expectations,
        \begin{align*}
            E[X|H_{1}] &= \frac{3 - 2p + p^{2}}{1 - p + p^{2}}\\
            E[X|T_{1}] &= \frac{2 + p^{2}}{1 - p + p^{2}}\\
            E[X] &= \frac{2 + p - p^{2}}{1 - p + p^{2}}
        \end{align*}
\end{document}